disk-betree/ImplModelCache.i.dfy
@@ -75,7 +75,39 @@ module ImplModelCache {
     getFreeRef2Iterate(s, avoid, 1)
   }
 
-  function {:opaque} write(k: Constants, s: Variables, ref: BT.G.Reference, node: Node)
+  // Bookkeeping only - we update the cache with the Node separately.
+  // This turns out to be easier to do.
+
+  function {:opaque} writeBookkeeping(k: Constants, s: Variables, ref: BT.G.Reference, children: Option<seq<BT.G.Reference>>)
+  : (s': Variables)
+  requires s.Ready?
+  ensures s'.Ready?
+  {
+    var eph := s.ephemeralIndirectionTable[ref := (None, if children.Some? then children.value else [])];
+    s.(ephemeralIndirectionTable := eph)
+        .(lru := LruModel.Use(s.lru, ref))
+  }
+
+  function {:opaque} allocBookkeeping(k: Constants, s: Variables, children: Option<seq<BT.G.Reference>>)
+  : (p: (Variables, Option<Reference>))
+  requires s.Ready?
+  ensures var (s', id) := p;
+    s'.Ready?
+  {
+    var ref := getFreeRef(s);
+    if ref.Some? then (
+      (writeBookkeeping(k, s, ref.value, children), ref)
+    ) else (
+      (s, None)
+    )
+  }
+
+  // fullWrite and fullAlloc are like writeBookkeeping/allocBookkeeping, except that fullWrite and fullAlloc update
+  // the cache with the node. In the implementation of betree operations we use the above,
+  // because it turns out to be easier to do the cache updates separately. However, for the proofs
+  // it is easier to use the below.
+
+  function writeWithNode(k: Constants, s: Variables, ref: BT.G.Reference, node: Node)
   : (s': Variables)
   requires s.Ready?
   ensures s'.Ready?
@@ -85,7 +117,7 @@ module ImplModelCache {
         .(lru := LruModel.Use(s.lru, ref))
   }
 
-  function {:opaque} alloc(k: Constants, s: Variables, node: Node)
+  function allocWithNode(k: Constants, s: Variables, node: Node)
   : (p: (Variables, Option<Reference>))
   requires s.Ready?
   ensures var (s', id) := p;
@@ -93,26 +125,24 @@ module ImplModelCache {
   {
     var ref := getFreeRef(s);
     if ref.Some? then (
-      (write(k, s, ref.value, node), ref)
+      (writeWithNode(k, s, ref.value, node), ref)
     ) else (
       (s, None)
     )
   }
- 
+
   lemma allocCorrect(k: Constants, s: Variables, node: Node)
   requires s.Ready?
   requires WFVars(s)
   requires WFNode(node)
   requires BC.BlockPointsToValidReferences(INode(node), IIndirectionTable(s.ephemeralIndirectionTable).graph)
   requires TotalCacheSize(s) <= MaxCacheSize() - 1
-  ensures var (s', ref) := alloc(k, s, node);
+  ensures var (s', ref) := allocWithNode(k, s, node);
     && WFVars(s')
     && (ref.Some? ==> BC.Alloc(Ik(k), IVars(s), IVars(s'), ref.value, INode(node)))
     && (ref.None? ==> s' == s)
     && (ref.Some? ==> TotalCacheSize(s') == TotalCacheSize(s) + 1)
   {
-    reveal_alloc();
-    reveal_write();
     var ref := getFreeRef(s);
     if ref.Some? {
       LruModel.LruUse(s.lru, ref.value);
@@ -127,17 +157,16 @@ module ImplModelCache {
   requires WFNode(node)
   requires BC.BlockPointsToValidReferences(INode(node), IIndirectionTable(s.ephemeralIndirectionTable).graph)
   requires s.frozenIndirectionTable.Some? && ref in s.frozenIndirectionTable.value ==> s.frozenIndirectionTable.value[ref].0.Some?
-  ensures var s' := write(k, s, ref, node);
+  ensures var s' := writeWithNode(k, s, ref, node);
     && WFVars(s')
     && BC.Dirty(Ik(k), IVars(s), IVars(s'), ref, INode(node))
     && TotalCacheSize(s') == TotalCacheSize(s)
   {
-    reveal_write();
     WeightBucketEmpty();
 
     LruModel.LruUse(s.lru, ref);
 
-    var s' := write(k, s, ref, node);
+    var s' := writeWithNode(k, s, ref, node);
     assert WFVars(s');
   }
  
@@ -148,12 +177,11 @@ module ImplModelCache {
   requires WFNode(node)
   requires TotalCacheSize(s) <= MaxCacheSize() - 1
   requires BC.BlockPointsToValidReferences(INode(node), IIndirectionTable(s.ephemeralIndirectionTable).graph)
-  ensures var s' := write(k, s, ref, node);
+  ensures var s' := writeWithNode(k, s, ref, node);
     && WFVars(s')
     && BC.Alloc(Ik(k), IVars(s), IVars(s'), ref, INode(node))
     && TotalCacheSize(s') == TotalCacheSize(s) + 1
   {
-    reveal_write();
     LruModel.LruUse(s.lru, ref);
   }
 
